# baseURI: http://www.bbc.co.uk/ontologies/creativework
# imports: http://purl.org/dc/elements/1.1/
# imports: http://www.bbc.co.uk/ontologies/provenance
# imports: http://purl.org/dc/terms/

@prefix bbc: <http://www.bbc.co.uk/ontologies/bbc/> .
@prefix dc: <http://purl.org/dc/elements/1.1/> .
@prefix dcterms: <http://purl.org/dc/terms/> .
@prefix owl: <http://www.w3.org/2002/07/owl#> .
@prefix rdf: <http://www.w3.org/1999/02/22-rdf-syntax-ns#> .
@prefix rdfs: <http://www.w3.org/2000/01/rdf-schema#> .
@prefix xsd: <http://www.w3.org/2001/XMLSchema#> .
@prefix bbc: <http://www.bbc.co.uk/ontologies/bbc/> .
@prefix cwork: <http://www.bbc.co.uk/ontologies/creativework/> .
@prefix core: <http://www.bbc.co.uk/ontologies/coreconcepts/> .
@prefix provenance: <http://www.bbc.co.uk/ontologies/provenance/> .
@prefix tagging: <http://www.bbc.co.uk/ontologies/tagging/> .

<http://www.bbc.co.uk/ontologies/creativework>
  rdf:type owl:Ontology , provenance:Ontology ;
  rdfs:comment "This is the model we use to express the minimum metadata necessary to express a piece of creative content in the platform. The creative work ontology is continuously evolving based on our clients' requirements. There is a core class in this model, which is the CreativeWork class and properties that support information the LDP clients need to build their products such as title, thumbnail, URL e.t.c."@en-gb ;
  rdfs:label "Creative Work Ontology"@en-gb ;
  dc:creator <mailto:LinkedData@bbc.co.uk> ;
  dc:date "2012-12-01"^^xsd:date ;
  dcterms:modified "2021-03-16"^^xsd:date ;
  dcterms:license <http://creativecommons.org/licenses/by/4.0/> ;
  provenance:canonicalLocation "https://github.com/bbc/ontologies/blob/master/core/creativework.ttl"^^xsd:string ;
  provenance:changeReason "genre & format --> subPropertyOf tagging ontology equivalents"@en-gb ;
  provenance:public "true"^^xsd:boolean ;
  provenance:slug "creativework"^^xsd:string ;
  provenance:version "1.19"^^xsd:string ;
  owl:imports <http://www.bbc.co.uk/ontologies/provenance> , dc: , dcterms: ;
  owl:priorVersion cwork:1.18 ;
  owl:versionIRI cwork:1.19 ;
  owl:versionInfo "1.19"^^xsd:string .

## Classes

cwork:Article
  rdf:type owl:Class ;
  rdfs:comment "This is the class of creative works that are associated with the Optimo service. This is to distinguish content published from Optimo from that produced by CPS."@en-gb ;
  rdfs:isDefinedBy <http://www.bbc.co.uk/ontologies/creativework/1.12> ;
  rdfs:label "Article"@en-gb ;
  rdfs:subClassOf cwork:CreativeWork .

cwork:Audience
  rdf:type owl:Class ;
  rdfs:comment "Enumerated class of the audiences the BBC creates content for."@en-gb ;
  rdfs:isDefinedBy <http://www.bbc.co.uk/ontologies/creativework> ;
  rdfs:label "Audience"@en-gb .

cwork:AudioFormat
  rdf:type cwork:Format ;
  rdfs:comment "Used to represent that the primary format of a CreativeWork is Audio."@en-gb ;
  rdfs:isDefinedBy <http://www.bbc.co.uk/ontologies/creativework> ;
  rdfs:label "AudioFormat"@en-gb .

cwork:BlogPost
  rdf:type owl:Class ;
  rdfs:comment "This is the class of creative works that are associated with particular journalists or correspondents. The analysis, commentary and personal viewpoint of the creator is reflected on the blog post and the blog post is usually associated prominently with the name of the creator. BlogPost can have different types of formats."@en-gb ;
  rdfs:isDefinedBy <http://www.bbc.co.uk/ontologies/creativework/1.4> ;
  owl:deprecated "true"^^xsd:boolean;
  rdfs:label "BlogPost"@en-gb ;
  rdfs:subClassOf cwork:CreativeWork .

cwork:Category
  rdf:type owl:Class ;
  rdfs:comment "A class to represent different categorisations of creative works from different clients. This class is instantiated in the clients' application logic models."@en-gb ;
  rdfs:isDefinedBy <http://www.bbc.co.uk/ontologies/creativework> ;
  rdfs:label "Category"@en-gb .

cwork:Clip
  rdf:type owl:Class ;
  rdfs:comment "The Clips subclass of programmes produced by the BBC."@en-gb ;
  rdfs:isDefinedBy <http://www.bbc.co.uk/ontologies/creativework/1.4> ;
  owl:deprecated "true"^^xsd:boolean;
  rdfs:label "Clip"@en-gb ;
  rdfs:subClassOf cwork:Programme .

cwork:CloseUpThumbnail
  rdf:type cwork:ThumbnailType ;
  rdfs:comment "A 16x9 image, focused and zoomed in one part of the image, usually when the standard thumbnail is very small to be meaningful (e.g., in mobile)."@en-gb ;
  rdfs:isDefinedBy <http://www.bbc.co.uk/ontologies/creativework> ;
  rdfs:label "CloseUpThumbnail"@en-gb .

cwork:Commentary
  rdf:type owl:Class ;
  rdfs:comment "This class represents short form creative works in the shape of updates. These differ from the other types of creative works because they haven't got independent URLs  as (primaryContentOf) from which they can be retrieved."@en-gb ;
  rdfs:isDefinedBy <http://www.bbc.co.uk/ontologies/creativework/1.4> ;
  owl:deprecated "true"^^xsd:boolean;
  rdfs:label "Commentary"@en-gb ;
  rdfs:subClassOf cwork:CreativeWork .

cwork:CreativeWork
  rdf:type owl:Class ;
  rdfs:comment "The class of creative works produced by the BBC."@en-gb ;
  rdfs:isDefinedBy <http://www.bbc.co.uk/ontologies/creativework> ;
  rdfs:label "CreativeWork"@en-gb ;
  rdfs:subClassOf owl:Thing .

cwork:ElectionAlert
  rdf:type owl:Class ;
  rdfs:comment "This class is used to describe creative works which are Election Alerts."@en-gb ;
  rdfs:isDefinedBy <http://www.bbc.co.uk/ontologies/creativework/1.13> ;
  rdfs:label "ElectionAlert"@en-gb ;
  rdfs:subClassOf cwork:CreativeWork .

cwork:Episode
  rdf:type owl:Class ;
  rdfs:comment "The Episodes subclass of programmes produced by the BBC."@en-gb ;
  rdfs:isDefinedBy <http://www.bbc.co.uk/ontologies/creativework/1.4> ;
  owl:deprecated "true"^^xsd:boolean;
  rdfs:label "Episode"@en-gb ;
  rdfs:subClassOf cwork:Programme .

cwork:FixedSize144Thumbnail
  rdf:type cwork:ThumbnailType ;
  rdfs:comment "Fixed size thumbnail"@en-gb ;
  rdfs:isDefinedBy <http://www.bbc.co.uk/ontologies/creativework/1.4> ;
  owl:deprecated "true"^^xsd:boolean;
  rdfs:label "FixedSize144Thumbnail"@en-gb .

cwork:FixedSize224Thumbnail
  rdf:type cwork:ThumbnailType ;
  rdfs:comment "Fixed size thumbnail"@en-gb ;
  rdfs:isDefinedBy <http://www.bbc.co.uk/ontologies/creativework/1.4> ;
  owl:deprecated "true"^^xsd:boolean;
  rdfs:label "FixedSize224Thumbnail"@en-gb .

cwork:FixedSize226Thumbnail
  rdf:type cwork:ThumbnailType ;
  rdfs:comment "Fixed size thumbnail"@en-gb ;
  rdfs:isDefinedBy <http://www.bbc.co.uk/ontologies/creativework/1.4> ;
  owl:deprecated "true"^^xsd:boolean;
  rdfs:label "FixedSize226Thumbnail"@en-gb .

cwork:FixedSize464Thumbnail
  rdf:type cwork:ThumbnailType ;
  rdfs:comment "Fixed size thumbnail"@en-gb ;
  rdfs:isDefinedBy <http://www.bbc.co.uk/ontologies/creativework/1.4> ;
  owl:deprecated "true"^^xsd:boolean;
  rdfs:label "FixedSize464Thumbnail"@en-gb .

cwork:FixedSize66Thumbnail
  rdf:type cwork:ThumbnailType ;
  rdfs:comment "Fixed size thumbnail"@en-gb ;
  rdfs:isDefinedBy <http://www.bbc.co.uk/ontologies/creativework/1.4> ;
  owl:deprecated "true"^^xsd:boolean;
  rdfs:label "FixedSize66Thumbnail"@en-gb .

cwork:Format
  rdf:type owl:Class ;
  rdfs:comment "The primary format of the CreativeWork and it can be one of the five instances. This is needed for selecting the appropriate icon with which to overlay the preview thumbnail of the creative work."@en-gb ;
  rdfs:isDefinedBy <http://www.bbc.co.uk/ontologies/creativework> ;
  rdfs:label "Format"@en-gb ;
  rdfs:subClassOf owl:Thing .

cwork:ImageFormat
  rdf:type cwork:Format ;
  rdfs:comment "Used to represent that the primary format of a CreativeWork is Image"@en-gb ;
  rdfs:isDefinedBy <http://www.bbc.co.uk/ontologies/creativework> ;
  rdfs:label "ImageFormat"@en-gb .

cwork:InteractiveFormat
  rdf:type cwork:Format ;
  rdfs:comment "Used to represent that the primary format of a CreativeWork is Interactive"@en-gb ;
  rdfs:isDefinedBy <http://www.bbc.co.uk/ontologies/creativework> ;
  rdfs:label "InteractiveFormat"@en-gb .

cwork:InternationalAudience
  rdf:type cwork:Audience ;
  rdfs:comment "The international (non UK) audience. The creative works linked to this instance are *only available to the international audience*."@en-gb ;
  rdfs:isDefinedBy <http://www.bbc.co.uk/ontologies/creativework> ;
  rdfs:label "InternationalAudience"@en-gb .

cwork:LiveCoverage
  rdf:type owl:Class ;
  rdfs:comment "This class is used to describe that creative works which are coverage of a live event. (Note that this isn't meant to describe the fact that the event is live currently. An example of a Live Coverage creative work is the live event page covering live the England VS Australia cricket match, last saturday's football matches or last year's elections)"@en-gb ;
  rdfs:isDefinedBy <http://www.bbc.co.uk/ontologies/creativework/1.4> ;
  owl:deprecated "true"^^xsd:boolean;
  rdfs:label "LiveCoverage"@en-gb ;
  rdfs:subClassOf cwork:CreativeWork .

cwork:TravelIncident
  rdf:type owl:Class ;
  rdfs:comment "This class is used to describe creative works which are Travel Incidents."@en-gb ;
  rdfs:isDefinedBy <http://www.bbc.co.uk/ontologies/creativework/1.10> ;
  rdfs:label "TravelIncident"@en-gb ;
  rdfs:subClassOf cwork:CreativeWork .

cwork:WeatherAlert
  rdf:type owl:Class ;
  rdfs:comment "This class is used to describe creative works which are Weather Alerts."@en-gb ;
  rdfs:isDefinedBy <http://www.bbc.co.uk/ontologies/creativework/1.10> ;
  rdfs:label "WeatherAlert"@en-gb ;
  rdfs:subClassOf cwork:CreativeWork .

cwork:LiveEventPage
  rdf:type owl:Class ;
  rdfs:comment "This class is created to support the LiveEventPages from CPS. This will be soon deprecated for the sake of LiveCoverage"@en-gb ;
  rdfs:isDefinedBy <http://www.bbc.co.uk/ontologies/creativework/1.4> ;
  owl:deprecated "true"^^xsd:boolean;
  rdfs:label "LiveEventPage"@en-gb ;
  rdfs:subClassOf cwork:CreativeWork .

cwork:MediaType
	a owl:Class ;
	rdfs:subClassOf tagging:MediaType ;
	rdfs:label "Media type"@en-gb ;
	rdfs:comment "A class to represent media types, e.g. audio, video, text etc"@en-gb ;
	rdfs:isDefinedBy cwork:1.17 .

cwork:NationalAudience
  rdf:type cwork:Audience ;
  rdfs:comment "The national audience. The creative works linked to this instance are *only available to the national audience*."@en-gb ;
  rdfs:isDefinedBy <http://www.bbc.co.uk/ontologies/creativework> ;
  rdfs:label "NationalAudience"@en-gb .

cwork:NewsItem
  rdf:type owl:Class ;
  rdfs:comment "The class of all news items that the BBC produces. They can be textual articles, or media asset pages (audio or video) or live coverage of events (use the liveCoverage property)."@en-gb ;
  rdfs:isDefinedBy <http://www.bbc.co.uk/ontologies/creativework/1.4> ;
  owl:deprecated "true"^^xsd:boolean;
  rdfs:label "NewsItem"@en-gb ;
  rdfs:subClassOf cwork:CreativeWork .

cwork:PictureGalleryFormat
  rdf:type cwork:Format ;
  rdfs:comment "Used to represent that the primary format of a CreativeWork is of PictureGallery (this is a mid-term solution for the modelling of galleries)"@en-gb ;
  rdfs:isDefinedBy <http://www.bbc.co.uk/ontologies/creativework> ;
  rdfs:label "PictureGalleryFormat"@en-gb .

cwork:Programme
  rdf:type owl:Class ;
  rdfs:comment "The class of programmes produced by the BBC"@en-gb ;
  rdfs:isDefinedBy <http://www.bbc.co.uk/ontologies/creativework/1.4> ;
  owl:deprecated "true"^^xsd:boolean;
  rdfs:label "Programme"@en-gb ;
  rdfs:subClassOf cwork:CreativeWork .

cwork:StandardThumbnail
  rdf:type cwork:ThumbnailType ;
  rdfs:comment "A 16x9 image used in most occasions"@en-gb ;
  rdfs:isDefinedBy <http://www.bbc.co.uk/ontologies/creativework> ;
  rdfs:label "StandardThumbnail"@en-gb .

cwork:TextualFormat
  rdf:type cwork:Format ;
  rdfs:comment "Used to represent that the primary format of a CreativeWork is Text"@en-gb ;
  rdfs:isDefinedBy <http://www.bbc.co.uk/ontologies/creativework> ;
  rdfs:label "TextualFormat"@en-gb .

cwork:Thumbnail
  rdf:type owl:Class ;
  rdfs:comment "Used to associate a Creative Work with the canonical location of the thumbnail. The URI of each of its instances is the full canonical location of the thumbnail"@en-gb ;
  rdfs:isDefinedBy <http://www.bbc.co.uk/ontologies/creativework> ;
  rdfs:label "Thumbnail"@en-gb ;
  rdfs:subClassOf owl:Thing .

cwork:ThumbnailType
  rdf:type owl:Class ;
  rdfs:comment "Enumerated class of the allowed thumbnail types"@en-gb ;
  rdfs:isDefinedBy <http://www.bbc.co.uk/ontologies/creativework> ;
  rdfs:label "ThumbnailType"@en-gb ;
  rdfs:subClassOf owl:Thing .

cwork:VideoFormat
  rdf:type cwork:Format ;
  rdfs:comment "Used to represent that the primary format of a CreativeWork is Video"@en-gb ;
  rdfs:isDefinedBy <http://www.bbc.co.uk/ontologies/creativework> ;
  rdfs:label "VideoFormat"@en-gb .


## Properties

cwork:about
  rdf:type owl:ObjectProperty ;
  rdfs:comment "Indicates that a BBC asset is about a tag concept"@en-gb ;
  rdfs:domain owl:Thing ;
  rdfs:isDefinedBy <http://www.bbc.co.uk/ontologies/creativework> ;
  rdfs:label "about"@en-gb ;
  rdfs:range tagging:TagConcept ;
  rdfs:subPropertyOf cwork:tag .

cwork:altText
  rdf:type owl:DatatypeProperty ;
  rdfs:comment "The alternative text for a thumbnail in case the URL is not resolved"@en-gb ;
  rdfs:domain cwork:Thumbnail ;
  rdfs:isDefinedBy <http://www.bbc.co.uk/ontologies/creativework> ;
  rdfs:label "altText"@en-gb ;
  rdfs:range xsd:string .

cwork:audience
  rdf:type owl:ObjectProperty ;
  rdfs:comment "Associates the Creative Work with an audience instance"@en-gb ;
  rdfs:domain cwork:CreativeWork ;
  rdfs:isDefinedBy <http://www.bbc.co.uk/ontologies/creativework> ;
  rdfs:label "audience"@en-gb ;
  rdfs:range cwork:Audience .

cwork:category
  rdf:type owl:ObjectProperty ;
  rdfs:comment "The category property is another mid term solution for maintaining the functionality supporting individual clients. For example, the type of gossip is something that the sports pal use for the moment. The values of the property are decided by the client teams in collaboration with LDP"@en-gb ;
  rdfs:domain cwork:CreativeWork ;
  rdfs:isDefinedBy <http://www.bbc.co.uk/ontologies/creativework> ;
  rdfs:label "category"@en-gb ;
  rdfs:range cwork:Category .

cwork:createdBy
  rdf:type owl:ObjectProperty ;
  rdfs:comment "associate a creative work with its creator"@en-gb ;
  rdfs:domain cwork:CreativeWork ;
  rdfs:isDefinedBy <http://www.bbc.co.uk/ontologies/creativework> ;
  rdfs:label "createdBy"@en-gb ;
  rdfs:range tagging:TagConcept .

cwork:dateCreated
  rdf:type owl:DatatypeProperty ;
  rdfs:comment "Date created of CreativeWork"@en-gb ;
  rdfs:domain cwork:CreativeWork ;
  rdfs:isDefinedBy <http://www.bbc.co.uk/ontologies/creativework> ;
  rdfs:label "dateCreated"@en-gb ;
  rdfs:range xsd:date .

cwork:dateModified
  rdf:type owl:DatatypeProperty ;
  rdfs:comment "Date modified of CreativeWork"@en-gb ;
  rdfs:domain cwork:CreativeWork ;
  rdfs:isDefinedBy <http://www.bbc.co.uk/ontologies/creativework> ;
  rdfs:label "dateModified"@en-gb ;
  rdfs:range xsd:date .

cwork:dateIssued
  rdf:type owl:DatatypeProperty ;
  rdfs:label "dateIssued"@en-gb ;
  rdfs:comment "The formal date of an asset's publication from the point of view of the audience"@en-gb ;
  rdfs:domain owl:Thing ;
  rdfs:range xsd:datetime ;
  rdfs:isDefinedBy cwork:1.17 .

cwork:dateFirstReleased
  rdf:type owl:DatatypeProperty ;
  rdfs:label "dateFirstReleased"@en-gb ;
  rdfs:comment "The date something was first broadcast or published by the BBC (or, for films, the date of UK cinematic release)"@en-gb ;
  rdfs:domain owl:Thing ;
  rdfs:range xsd:datetime ;
  rdfs:isDefinedBy cwork:1.19 .

cwork:dateLastReleased
  rdf:type owl:DatatypeProperty ;
  rdfs:label "dateLastReleased"@en-gb ;
  rdfs:comment "The date something was most recently published (including minor updates) or most recently broadcast (including unadvertised repeats)"@en-gb ;
  rdfs:domain owl:Thing ;
  rdfs:range xsd:datetime ;
  rdfs:isDefinedBy cwork:1.19 .

cwork:description
  rdf:type owl:DatatypeProperty ;
  rdfs:comment "The description of the Creative Work"@en-gb ;
  rdfs:domain cwork:CreativeWork ;
  rdfs:isDefinedBy <http://www.bbc.co.uk/ontologies/creativework> ;
  rdfs:label "description"@en-gb ;
  rdfs:range xsd:string .

cwork:format
  rdf:type owl:ObjectProperty ;
  rdfs:comment "Associates a BBC asset with a bbc:Format instance" ;
  rdfs:domain owl:Thing ;
  rdfs:range bbc:Format ;
  rdfs:isDefinedBy <http://www.bbc.co.uk/ontologies/creativework> ;
  rdfs:label "format"@en-gb ;
  rdfs:subPropertyOf tagging:format .

cwork:genre
  rdf:type owl:ObjectProperty ;
  rdfs:comment "Associates a BBC asset with a bbc:Genre instance" ;
  rdfs:domain owl:Thing ;
  rdfs:range bbc:Genre ;
  rdfs:isDefinedBy <http://www.bbc.co.uk/ontologies/creativework> ;
  rdfs:label "genre"@en-gb ;
  rdfs:subPropertyOf tagging:genre .

cwork:language
  rdf:type owl:DatatypeProperty ;
  rdfs:comment "The language of the creative work, please use BCP47 https://tools.ietf.org/html/bcp47"@en-gb ;
  rdfs:domain cwork:CreativeWork ;
  rdfs:isDefinedBy <http://www.bbc.co.uk/ontologies/creativework> ;
  rdfs:label "language"@en-gb ;
  rdfs:range xsd:language .

cwork:mentions
  rdf:type owl:ObjectProperty ;
  rdfs:comment "Indicates that a BBC asset mentions a tag concept"@en-gb ;
  rdfs:domain owl:Thing ;
  rdfs:isDefinedBy <http://www.bbc.co.uk/ontologies/creativework> ;
  rdfs:label "mentions"@en-gb ;
  rdfs:range tagging:TagConcept ;
  rdfs:subPropertyOf cwork:tag .

cwork:primaryFormat
  rdf:type owl:ObjectProperty ;
  rdfs:comment "Associates the Creative Work with the Primary Format instance"@en-gb ;
  rdfs:domain cwork:CreativeWork ;
  rdfs:isDefinedBy <http://www.bbc.co.uk/ontologies/creativework> ;
  rdfs:label "primaryFormat"@en-gb ;
  rdfs:range cwork:Format .

cwork:shortTitle
  rdf:type owl:DatatypeProperty ;
  rdfs:comment "The sort title of the Creative Work"@en-gb ;
  rdfs:domain cwork:CreativeWork ;
  rdfs:isDefinedBy <http://www.bbc.co.uk/ontologies/creativework> ;
  rdfs:label "shortTitle"@en-gb ;
  rdfs:range xsd:string .

cwork:tag
  rdf:type owl:ObjectProperty ;
  rdfs:comment "Indicates that the creative work is tagged with tag concept"@en-gb ;
  rdfs:domain cwork:CreativeWork ;
  rdfs:isDefinedBy <http://www.bbc.co.uk/ontologies/creativework> ;
  rdfs:label "tag"@en-gb ;
  rdfs:range tagging:TagConcept .

cwork:thumbnail
  rdf:type owl:ObjectProperty ;
  rdfs:comment "Associates the Creative Work with the Thumbnail instance"@en-gb ;
  rdfs:domain cwork:CreativeWork ;
  rdfs:isDefinedBy <http://www.bbc.co.uk/ontologies/creativework> ;
  rdfs:label "thumbnail"@en-gb ;
  rdfs:range cwork:Thumbnail .

cwork:thumbnailType
  rdf:type owl:ObjectProperty ;
  rdfs:comment "Associates the Thumbnail instance with a Thumbnail type"@en-gb ;
  rdfs:domain cwork:Thumbnail ;
  rdfs:isDefinedBy <http://www.bbc.co.uk/ontologies/creativework> ;
  rdfs:label "thumbnailType"@en-gb ;
  rdfs:range cwork:ThumbnailType .

cwork:title
  rdf:type owl:DatatypeProperty ;
  rdfs:comment "The title of the Creative Work"@en-gb ;
  rdfs:domain cwork:CreativeWork ;
  rdfs:isDefinedBy <http://www.bbc.co.uk/ontologies/creativework> ;
  rdfs:label "title"@en-gb ;
  rdfs:range xsd:string .
